path_ORAM/tree.dfy
@@ -1,0 +1,96 @@
+datatype data = Data(data: string) | Dummy
+
+class Block {
+    var addr: nat
+    var data: data
+    
+    constructor(addr: nat, data: data)
+    {
+        this.addr := addr;
+        this.data := data;
+    }
+}
+
+
+class Bucket {
+    var blocks: array<Block>
+
+    constructor(bucketSize: nat, newAddr: nat)
+    {
+        var d := new Block(0, Data(""));
+        blocks := new Block[bucketSize](_ => d);
+        new;
+        var i: nat := 0;
+        var addr := newAddr;
+        while i < bucketSize
+            modifies blocks
+        {
+            blocks[i] := new Block(addr, Data(""));
+            addr := addr + 1;
+            i := i + 1;
+        }
+    }
+}
+
+
+class Tree {
+    var buckets: array<Bucket>
+    // Access pattern buffers
+    var bufferR: seq<(string, nat)> // Read operations log
+    var bufferW: seq<(string, nat)> // Write operations log
+
+    constructor(treeSize: nat, bucketSize: nat)
+    {
+        var d := new Bucket(bucketSize, 0);
+        buckets := new Bucket[treeSize](_ => d);
+        bufferR := [];
+        bufferW := [];
+        
+        new;
+
+        var i: nat := 0;
+        var addr: nat := 0;
+        while i < treeSize
+            modifies buckets
+        {
+            buckets[i] := new Bucket(bucketSize, addr);
+            addr := addr + bucketSize;
+            i := i + 1;
+        }
+    }
+
+    method ReadBucket(bucket: nat) returns (blocks: seq<Block>)
+        modifies this`bufferR
+        ensures bufferR == old(bufferR) + [("R", bucket)]
+    {
+        // Log the read operation
+        bufferR := bufferR + [("R", bucket)];
+    }
+
+    method WriteBucket(bucket: nat, blocks: seq<Block>)
+        modifies this`buckets, this`bufferW
+        ensures bufferW == old(bufferW) + [("W", bucket)]
+    {
+        // Log the write operation
+        bufferW := bufferW + [("W", bucket)];
+    }
+
+    method WriteAccessLog()
+        requires |bufferR| >= 0 && |bufferW| >= 0
+        modifies this`bufferR, this`bufferW
+        ensures |bufferR| == 0 && |bufferW| == 0
+    {
+        // In a real implementation, this would write to a file
+        // For verification purposes, we just clear the buffers
+        ClearBuffers();
+    }
+
+    method ClearBuffers()
+        modifies this`bufferR, this`bufferW
+        ensures |bufferR| == 0
+        ensures |bufferW| == 0
+    {
+        bufferR := [];
+        bufferW := [];
+    }
+}
